# Identities Index

## Arithmetic Addition and Subtraction Identities

|  |  |  |
|---|---|---|
| $a-(b\color{red}-\color{black}c)=a-b\color{red}+\color{black}c$ |  |  |
|  |  |  |

## Arithmetic Multiplicative and Division identities

A negative times a negative is always a positive. As in $\color{red}-\color{black}1\times\color{red}-\color{black}1=1$.  
A positive times a negative is a negative. As in $\color{red}-\color{black}1\times1=\color{red}-\color{black}1$.  

|  |  |  |
|---|---|---|
| $0a=0$ |  |  |
| $1a=a$ |  |  |
| $(−1)a=−a$ |  |  |
| $(ab)c=a(bc)$ |  |  |
| $ab + ac=a(b + c)$ <br /> $(a + b)c=ac + bc$ |  |  |
|  |  |  |

## Expansion and Distribution Identities

|  |  |  |
|---|---|---|
| $c(a+b)=ca+cb$ |  |  |
| $c(ac+bc)=ac^2+bc^2$ |  |  |
| $(a+b)^2=a^2+2ab+b^2$ |  |  |
| $(a-b)^2=a^2-2ab+b^2$ |  |  |
| $(a+b)(c+d)=ac+ad+bc+bd$ |  |  |
| $(a-b)(c-d)=ac-ad-bc+bd$ |  |  |
| $(a+b)(c-d)=ac-ad+bc-bd$ |  |  |
| $(a-b)(c+d)=ac+ad-bc-bd$ |  |  |
| $\frac{\frac{a}{b}}{b}=\frac{a}{b^2}$ |  |  |
|  |  |  |

## Radical and Exponential Identities

|  |  |  |
|---|---|---|
| $1^n=1;$ |  | One times another one is always one. |
| $a^0=1$ |  | When the exponent is 0 it equals 1. |
| $a\color{red}^1\color{black}=a$ |  | For exponents of 1, the exponent is dropped |
| $a^{m}a^{n}=a^{m+n}, a ≠ 0, a ≠ m, n ≥ 0$ |  |  |
| $(a^m)^n=a^{mn}, a ≠ 0, a ≠ m ≥ 0$ |  |  |
| $(ab)^n=a^nb^n;$ |  |  |
| $a^{−1}=\frac{1}{a}$ |  |  |
| $x^{-a}=\frac{1}{x^a}$ |  |  |
| $x^{(a/b)}=\sqrt[b]{x a} \sqrt[b]{x}^a$ |  |  |
| $x^{a - b}=\frac{x^a}{x^b}$ |  |  |
| $\sqrt{a^2}=\|a\|$ |  |  |
| $\sqrt{a}\sqrt{a}=a$ |  |  |
| $\sqrt{a}\sqrt{b}=\sqrt{ab}$ |  |  |
| $\sqrt{\frac{a}{b}}=\frac{\sqrt{a}}{\sqrt{b}}$ |  |  |
| $\sqrt{a^n}=(\sqrt{a})^n$ |  |  |
| $x^{\frac{m}{n}}=\sqrt[n]{x^m}=(\sqrt[n]{x})^m$ |  |  |
| $\sqrt{a}=a^{\frac{1}{2}}$ |  |  |
|  |  |  |

## Logarithm Identities

|  |  |  |
|---|---|---|
| $y = \log_b(x)$ |  | If and only if $x=b^y$ |
| $\log_b(1) = 0$ |  |  |
| $\log_b(b) = 1$ |  |  |
| $\log_b(xy) = \log_b(x) + \log_b(y)$ |  |  |
| $\log_b(\frac{x}{y}) = \log_b(x) - \log_b(y)$ |  |  |
| $\log_b(x^n) = n \log_b(x)$ |  |  |
| $\log_b(x) = \log_b(c)\log_c(x) = \frac{\log_c(x)}{\log_c(b)}$ |  |  |

## Trigonometric Identities

<center>
<svg width="111" height="66">
  <g stroke-width="1" stroke="black" fill="transparent">
 <polygon points="100,0  0,50 100,50" id="Triangle" />
 <polyline points="95,50  95,45 100,45" id="Right Angle" />
 <path d="M100 10 A 15 12 0 0 1 90 5" id="Cos Angle" />
 <path d="M12 50 A 15 12 0 0 0 11 45" id="Sin Angle" />
  </g>
  <g fill="black" font-family="san-serif" font-size="14">
 <text x="40" y="20" text-anchor="middle" id="c Letter">c</text>
 <text x="105" y="30" text-anchor="left" id="a Letter">a</text>
 <text x="55" y="65" text-anchor="middle" id="b Letter">b</text>
 <text x="25" y="48" text-anchor="left" id="theta Letter">θ</text>
 <text x="88" y="20" text-anchor="right" id="phi Letter">ɸ</text>
  </g>
</svg>
</center>

[Neat Visualization of Sine Cosine](https://1ucasvb.tumblr.com/post/79557434791/the-sine-and-cosine-functions-for-the-circle-as)

| Equation | Name | Description |
|:---:|---|---|
| $\sin{(0)}=0$ |  |  |
| $\cos{(0)}=1$ |  |  |
| $\sin(-\theta)=-\sin(\theta)$ | Change of Sign Odd Sine Identity. |  |
| $\cos(-\theta)=\cos(\theta)$ | Change of Sign Even Cosine Identity. |  |
| $\tan(-\theta)=-\tan(\theta)$ | Change of Sign Odd Tangent Identity. |  |
| $\csc(-\theta)=-\csc(\theta)$ | Change of Sign Odd Cosecant Identity. |  |
| $\sec(-\theta)=\sec(\theta)$ | Change of Sign Even Secant Identity. |  |
| $\cot(-\theta)=-\cot(\theta)$ | Change of Sign Odd Cotangent Identity. |  |
| $\sin(\theta)=\frac{1}{\csc(\theta)}=\frac{a}{c}$ | Sine Basic Identities. |  |
| $\cos(\theta)=\frac{1}{\sec(\theta)}=\frac{b}{c}$ | Cosine Basic Identities. |  |
| $\tan(\theta)=\frac{1}{\cot(\theta)}=\frac{\sin(\theta)}{\cos(\theta)}=\frac{a}{b}$ | Tangent Basic Identity. |  |
| $\csc(\theta)=\frac{1}{\sin(\theta)}=\frac{c}{a}$ | Cosecant Basic  Identity. |  |
| $\sec(\theta)=\frac{1}{\cos(\theta)}=\frac{c}{b}$ | Secant Basic Identity. |  |
| $\cot(\theta)=\frac{1}{tan(\theta)}=\frac{\cos(\theta)}{\sin(\theta)}=\frac{b}{a}$ | Cotangent Basic Identity. |  |
| $\frac{a}{\sin(A)}=\frac{b}{\sin(B)}=\frac{c}{\sin(C)}$ | Law of Sines Identities. |  |
| $a^{2}=b^{2}+c^{2}-2bc\cos(A)$ </br> $b^{2}=a^{2}+c^{2}-2ac\cos(B)$ </br> $c^{2}=a^{2}+b^{2}-2ab\cos(C)$ | Law of Cosines Identities. |  |
| $\frac{a-b}{a+ b}= \frac{\tan(\frac{A-B}{2})}{\tan(\frac{A+B}{2})}$ | Law of Tangents Identity. |  |
| $\sin^{2}(\theta)+\cos^{2}(\theta) = 1$ | Sine Cosign Pythagorean Identity. |  |
| $\tan^{2}(\theta)+1=\sec^{2}(\theta)$ | Tangent Secant Pythagorean Identity. |  |
| $\cot^{2}(\theta)+1=\csc^{2}(\theta)$ | Cotangent Cosecant Pythagorean Identity. |  |
| $\sin(\theta_1\pm\theta_2)=\sin(\theta_1)\cos(\theta_2)\pm\cos(\theta_1)\sin(\theta_2)$ <br /> $\sin(\theta_1+\theta_2)=\sin(\theta_1)\cos(\theta_2)+\cos(\theta_1)\sin(\theta_2)$ <br /> $\sin(\theta_1-\theta_2)=\sin(\theta_1)\cos(\theta_2)-\cos(\theta_1)\sin(\theta_2)$ | Sine Sum Difference Identities. |  |
| $\cos(\theta_1\pm\theta_2)=\cos(\theta_1)\cos(\theta_2)\mp\sin(\theta_1)\sin(\theta_2)$ <br /> $\cos(\theta_1+\theta_2)=\cos(\theta_1)\cos(\theta_2)-\sin(\theta_1)\sin(\theta_2)$ <br /> $\cos(\theta_1-\theta_2)=\cos(\theta_1)\cos(\theta_2)+\sin(\theta_1)\sin(\theta_2)$ | Cosine Sum Difference Identities. |  |
| $\sin{(\theta+\pi)}=-\sin{(\theta)}$ |  |  |
| $\cos{(\theta+\pi)}=-\cos{(\theta)}$ |  |  |
| $\tan(\theta_1\pm\theta_2)=\frac{\tan(\theta_1)\pm\tan(\theta_2)}{1\mp\tan(\theta_1)\tan(\theta_2)}$ <br /> $\tan(\theta_1+\theta_2)=\frac{\tan(\theta_1)+\tan(\theta_2)}{1-\tan(\theta_1)\tan(\theta_2)}$ <br /> $\tan(\theta_1-\theta_2)=\frac{\tan(\theta_1)-\tan(\theta_2)}{1+\tan(\theta_1)\tan(\theta_2)}$ | Tangent Sum Difference Identities. |  |
| $\sin(2\theta)=2\sin(\theta )\cos(\theta )$ | Double Angle Sine Identity. |  |
| $\cos(2\theta)=\cos^{2}(\theta)-\sin^{2}(\theta)=2\cos^{2}(\theta)-1=1-2\sin^{2}(\theta)$ | Cosine Double Angle Identity. |  |
| $\tan(2\theta)=\frac{2\tan(\theta)}{1-\tan^{2}(\theta)}$ | Tangent Double Angle Identity. |  |
| $\sin{(\frac{\theta}{2})}=\pm\sqrt{\frac{1-\cos{(\theta)}}{2}}$ <br /> $\sin^2(\theta)=\frac{1}{2}-\frac{1}{2}\cos(2\theta)=\frac{1}{2}[1-\cos(2\theta)]$ | Sine Half angle Identities. |  |
| $\cos{(\frac{\theta}{2})}=\pm\sqrt{\frac{1+\cos{(\theta)}}{2}}$ <br /> $\cos^2(\theta)=\frac{1}{2}+\frac{1}{2}\cos(2\theta)=\frac{1}{2}[1+\cos(2\theta)]$ | Cosine Half angle Identities. |  |
| $\tan{(\frac{\theta}{2})}=\pm\sqrt{\frac{1-\cos{(\theta)}}{1+\cos{(\theta)}}}=\frac{1-\cos{(\theta)}}{sin{(\theta)}}=\frac{\sin{(\theta)}}{1+\cos{(\theta)}}$ <br /> $\tan^2{(\theta)}=\frac{1-\cos{(\theta)}}{1+\cos{(\theta)}}$ | Tangent Half angle Identities. |  |
| $\sin(\theta_1)+\sin(\theta_2)=2\sin(\frac{\theta_1+\theta_2}{2})\cos(\frac{\theta_1−\theta_2}{2})$ | Sum of Sines Identity. |  |
| $\sin(\theta_1)-\sin(\theta_2)=2\cos{(\frac{\theta_1+\theta_2}{2})}\sin{(\frac{\theta_1-\theta_2}{2})}$ | Difference of Sines Identity. |  |
| $\cos(\theta_1)+\cos(\theta_2)=2\cos(\frac{\theta_1+\theta_2}{2})\cos(\frac{\theta_1-\theta_2}{2})$ | Sum of Cosines Identity. |  |
| $\cos(\theta_1)-\cos(\theta_2)=-2\sin(\frac{\theta_1+\theta_2}{2})\sin(\frac{\theta_1-\theta_2}{2})$ | Difference of Cosines Identity. |  |
| $\sin(\theta_1)\cos(\theta_2)=\frac{\sin(\theta_1+\theta_2)+\sin(\theta_1−\theta_2)}{2}$ | Product of Sine Cosine Identity. |  |
| $\cos(\theta_1)\sin(\theta_2)=\frac{\sin(\theta_1+\theta_2)-\sin(\theta_1−\theta_2)}{2}$ | Product of Cosine Sine identity. |  |
| $\cos(\theta_1)\cos(\theta_2)=\frac{\cos(\theta_1-\theta_2)+\cos(\theta_1+\theta_2)}{2}$ | Product of two Cosines Identity. |  |
| $\sin(\theta_1)\sin(\theta_2)=\frac{\cos(\theta_1−\theta_2)−\cos(\theta_1+\theta_2)}{2}$ | Product of two Sines Identity. |  |
| $\sin\left(3\theta\right)=-\sin ^3\left(\theta\right)+3\cos ^2\left(\theta\right)\sin \left(\theta\right)=-4\sin ^3\left(\theta\right)+3\sin \left(\theta\right)$ | Triple Angle Sine Identities. |  |
| $\cos \left(3\theta\right)=\cos ^3\left(\theta\right)-3\sin ^2\left(\theta\right)\cos \left(\theta\right)=4\cos ^3\left(\theta\right)-3\cos \left(\theta\right)$ | Triple Angle Cosine Identities. |  |
| $\tan \left(3\theta\right)=\frac{3\tan \left(\theta\right)-\tan ^3\left(\theta\right)}{1-3\tan ^2\left(\theta\right)}$ | Triple Angle Tangent Identity. |  |
| $\cot \left(3\theta\right)=\frac{3\cot \left(\theta\right)-\cot ^3\left(\theta\right)}{1-3\cot ^2\left(\theta\right)}$ | Triple Agent Cotangent Identity. |  |
